<?xml version="1.0" encoding="utf-8"?>
<rdf:RDF xmlns:dct="http://purl.org/dc/terms/"
  xmlns:owl="http://www.w3.org/2002/07/owl#" xmlns:rdf="http://www.w3.org/1999/02/22-rdf-syntax-ns#"
  xmlns:rdfs="http://www.w3.org/2000/01/rdf-schema#" xmlns:skos="http://www.w3.org/2004/02/skos/core#"
  xml:base="http://www.w3.org/2004/02/skos/core">
  <!-- This schema represents a formalisation of a subset of the semantic conditions
    described in the SKOS Reference document dated 18 August 2009, accessible
    at http://www.w3.org/TR/2009/REC-skos-reference-20090818/. XML comments of the form Sn are used to
    indicate the semantic conditions that are being expressed. Comments of the form
    [Sn] refer to assertions that are, strictly speaking, redundant as they follow
    from the RDF(S) or OWL semantics.

    A number of semantic conditions are *not* expressed formally in this schema. These are:

    S12
    S13
    S14
    S27
    S36
    S46

    For the conditions listed above, rdfs:comments are used to indicate the conditions.

   -->
  <owl:Ontology rdf:about="http://www.w3.org/2004/02/skos/core">
    <dct:title xml:lang="en">SKOS Vocabulary</dct:title>
		<dct:title xml:lang="sv">SKOS begreppsmodell</dct:title>
    <dct:contributor>Dave Beckett</dct:contributor>
    <dct:contributor>Nikki Rogers</dct:contributor>
    <dct:contributor>Participants in W3C's Semantic Web Deployment Working Group.</dct:contributor>
    <dct:description xml:lang="en">An RDF vocabulary for describing the basic structure and content of concept schemes such as thesauri, classification schemes, subject heading lists, taxonomies, 'folksonomies', other types of controlled vocabulary, and also concept schemes embedded in glossaries and terminologies.</dct:description>
    <dct:description xml:lang="sv">En RDF-vokabulär för att beskriva grundläggande struktur och innehåll i begreppsmodeller såsom tesaurusar, klassifikationsscheman, ämnesordsförteckningar, taxonomier, folksonomier och andra typer av kontrollerade ordlistor. Omfattar även sådana begreppsmodeller som finns inlemmade i ordlistor och terminologier.</dct:description>
    <dct:creator>Alistair Miles</dct:creator>
    <dct:creator>Sean Bechhofer</dct:creator>
    <rdfs:seeAlso rdf:resource="http://www.w3.org/TR/skos-reference/"/>
  </owl:Ontology>
  <rdf:Description rdf:about="#Concept">
    <rdfs:label xml:lang="en">Concept</rdfs:label>
    <rdfs:label xml:lang="sv">Begrepp</rdfs:label>
    <rdfs:isDefinedBy rdf:resource="http://www.w3.org/2004/02/skos/core"/>
    <skos:definition xml:lang="en">An idea or notion; a unit of thought.</skos:definition>
    <skos:definition xml:lang="sv">En abstrakt idé eller föreställning om något. Kunskapsenhet.</skos:definition>
    <!-- S1 -->
    <rdf:type rdf:resource="http://www.w3.org/2002/07/owl#Class"/>
  </rdf:Description>
  <rdf:Description rdf:about="#ConceptScheme">
    <rdfs:label xml:lang="en">Concept Scheme</rdfs:label>
    <rdfs:label xml:lang="sv">begreppsmodell</rdfs:label>
    <rdfs:isDefinedBy rdf:resource="http://www.w3.org/2004/02/skos/core"/>
    <skos:definition xml:lang="en">A set of concepts, optionally including statements about semantic relationships between those concepts.</skos:definition>
    <skos:definition xml:lang="sv">En uppsättning begrepp som även kan innehålla beskrivningar av deras inbördes relationer.</skos:definition>

    <skos:scopeNote xml:lang="en">A concept scheme may be defined to include concepts from different sources.</skos:scopeNote>
    <skos:scopeNote xml:lang="sv">En begreppsmodell kan även designas så att den innehåller begrepp från andra källor.</skos:scopeNote>
    <skos:example xml:lang="en">Thesauri, classification schemes, subject heading lists, taxonomies, 'folksonomies', and other types of controlled vocabulary are all examples of concept schemes. Concept schemes are also embedded in glossaries and terminologies.</skos:example>
    <skos:example xml:lang="sv">Tesaurusar, klassifikationsscheman, ämnesordsförteckningar, taxonomier, folksonomier och andra typer av kontrollerade ordlistor är samtliga exempel på begrepssystem. Begreppsmodeller kan även vara ingå i ordlistor och terminologier.</skos:example>
    <!-- S2 -->
    <rdf:type rdf:resource="http://www.w3.org/2002/07/owl#Class"/>
    <!-- S9 -->
    <owl:disjointWith rdf:resource="#Concept"/>
  </rdf:Description>
  <rdf:Description rdf:about="#Collection">
    <rdfs:label xml:lang="en">Collection</rdfs:label>
    <rdfs:label xml:lang="sv">Samling</rdfs:label>
    <rdfs:isDefinedBy rdf:resource="http://www.w3.org/2004/02/skos/core"/>
    <skos:definition xml:lang="en">A meaningful collection of concepts.</skos:definition>
    <skos:definition xml:lang="sv">En meningsfull samling av begrepp.</skos:definition>
    <skos:scopeNote xml:lang="en">Labelled collections can be used where you would like a set of concepts to be displayed under a 'node label' in the hierarchy.</skos:scopeNote>
    <skos:scopeNote xml:lang="sv">Namngivna samlingar kan användas ihop med semantiska relationer som t.ex. skos:narrower när man vill presentera en uppsättning begrepp under en "nodetikett" i en hierarki.</skos:scopeNote>
    <!-- S28 -->
    <rdf:type rdf:resource="http://www.w3.org/2002/07/owl#Class"/>
    <!-- S37 -->
    <owl:disjointWith rdf:resource="#Concept"/>
    <!-- S37 -->
    <owl:disjointWith rdf:resource="#ConceptScheme"/>
  </rdf:Description>
  <rdf:Description rdf:about="#OrderedCollection">
    <rdfs:label xml:lang="en">Ordered Collection</rdfs:label>
    <rdfs:label xml:lang="sv">Ordnad samling</rdfs:label>
    <rdfs:isDefinedBy rdf:resource="http://www.w3.org/2004/02/skos/core"/>
    <skos:definition xml:lang="en">An ordered collection of concepts, where both the grouping and the ordering are meaningful.</skos:definition>
    <skos:definition xml:lang="sv">En ordnat samling begrepp där både ordningen och grupperingen av begrepp har betydelse.</skos:definition>
    <skos:scopeNote xml:lang="en">Ordered collections can be used where you would like a set of concepts to be displayed in a specific order, and optionally under a 'node label'.</skos:scopeNote>
    <skos:scopeNote xml:lang="sv">En ordnad samling kan användas ihop med semantiska relationer när man vill att en samling begrepp ska presenteras i en viss ordning, eventuellt tillsammans med presentation under en "nodetikett".</skos:scopeNote>
    <!-- S28 -->
    <rdf:type rdf:resource="http://www.w3.org/2002/07/owl#Class"/>
    <!-- S29 -->
    <rdfs:subClassOf rdf:resource="#Collection"/>
  </rdf:Description>
  <rdf:Description rdf:about="#inScheme">
    <rdfs:label xml:lang="en">is in scheme</rdfs:label>
    <rdfs:label xml:lang="sv">ingår i modell</rdfs:label>
    <rdfs:isDefinedBy rdf:resource="http://www.w3.org/2004/02/skos/core"/>
    <skos:definition xml:lang="en">Relates a resource (for example a concept) to a concept scheme in which it is included.</skos:definition>
    <skos:definition xml:lang="sv">Kopplar en resurs (t.ex. ett begrepp) till en begreppsmodell i vilken den ingår.</skos:definition>
    <skos:scopeNote xml:lang="en">A concept may be a member of more than one concept scheme.</skos:scopeNote>
    <skos:scopeNote xml:lang="sv">Ett begrepp kan ingå i flera begreppsmodeller.</skos:scopeNote>
    <!-- S3 -->
    <rdf:type rdf:resource="http://www.w3.org/2002/07/owl#ObjectProperty"/>
    <!-- S4 -->
    <rdfs:range rdf:resource="#ConceptScheme"/>
    <!-- For non-OWL aware applications -->
    <rdf:type rdf:resource="http://www.w3.org/1999/02/22-rdf-syntax-ns#Property"/>
  </rdf:Description>
  <rdf:Description rdf:about="#hasTopConcept">
    <rdfs:label xml:lang="en">has top concept</rdfs:label>
    <rdfs:label xml:lang="sv">har huvudbegrepp</rdfs:label>
    <rdfs:isDefinedBy rdf:resource="http://www.w3.org/2004/02/skos/core"/>
    <skos:definition xml:lang="en">Relates, by convention, a concept scheme to a concept which is topmost in the broader/narrower concept hierarchies for that scheme, providing an entry point to these hierarchies.</skos:definition>
    <skos:definition xml:lang="sv">Kopplar en begreppsmodell till ett begrepp som är överst i hierarkin i modellen.</skos:definition>
    <!-- S3 -->
    <rdf:type rdf:resource="http://www.w3.org/2002/07/owl#ObjectProperty"/>
    <!-- S5 -->
    <rdfs:domain rdf:resource="#ConceptScheme"/>
    <!-- S6 -->
    <rdfs:range rdf:resource="#Concept"/>
    <!-- S8 -->
    <owl:inverseOf rdf:resource="#topConceptOf"/>
    <!-- For non-OWL aware applications -->
    <rdf:type rdf:resource="http://www.w3.org/1999/02/22-rdf-syntax-ns#Property"/>
  </rdf:Description>
  <rdf:Description rdf:about="#topConceptOf">
    <rdfs:label xml:lang="en">is top concept in scheme</rdfs:label>
    <rdfs:label xml:lang="sv">är huvudbegrepp i modellen</rdfs:label>
    <rdfs:isDefinedBy rdf:resource="http://www.w3.org/2004/02/skos/core"/>
    <skos:definition xml:lang="en">Relates a concept to the concept scheme that it is a top level concept of.</skos:definition>
    <skos:definition xml:lang="sv">Kopplar ett begrepp till en begreppsmodell för vilket begreppet är huvudbegrepp.</skos:definition>
    <!-- S3 -->
    <rdf:type rdf:resource="http://www.w3.org/2002/07/owl#ObjectProperty"/>
    <!-- S7 -->
    <rdfs:subPropertyOf rdf:resource="#inScheme"/>
    <!-- S8 -->
    <owl:inverseOf rdf:resource="#hasTopConcept"/>
    <!-- For non-OWL aware applications -->
    <rdf:type rdf:resource="http://www.w3.org/1999/02/22-rdf-syntax-ns#Property"/>
    <rdfs:domain rdf:resource="#Concept"/>
    <rdfs:range rdf:resource="#ConceptScheme"/>
  </rdf:Description>
  <rdf:Description rdf:about="#prefLabel">
    <rdfs:label xml:lang="en">preferred label</rdfs:label>
    <rdfs:label xml:lang="sv">föredragen term</rdfs:label>
    <rdfs:isDefinedBy rdf:resource="http://www.w3.org/2004/02/skos/core"/>
    <skos:definition xml:lang="en">The preferred lexical label for a resource, in a given language.</skos:definition>
    <skos:definition xml:lang="sv">Den föredragna termen för en resurs på ett visst språk.</skos:definition>
    <!-- S10 -->
    <rdf:type rdf:resource="http://www.w3.org/2002/07/owl#AnnotationProperty"/>
    <!-- S11 -->
    <rdfs:subPropertyOf rdf:resource="http://www.w3.org/2000/01/rdf-schema#label"/>
    <!-- S14 (not formally stated) -->
    <rdfs:comment xml:lang="en">A resource has no more than one value of skos:prefLabel per language tag, and no more than one value of skos:prefLabel without language tag.</rdfs:comment>
    <rdfs:comment xml:lang="sv">En resurs har maximalt en skos:prefLabel per språk och en skos:prefLabel utan språkangivelse.</rdfs:comment>
    <!-- S12 (not formally stated) -->
    <rdfs:comment xml:lang="en">The range of skos:prefLabel is the class of RDF plain literals.</rdfs:comment>
    <rdfs:comment xml:lang="sv">Omfattningen av skos:prefLabel är klassen RDF plain literals.</rdfs:comment>
    <!-- S13 (not formally stated) -->
    <rdfs:comment xml:lang="en">skos:prefLabel, skos:altLabel and skos:hiddenLabel are pairwise disjoint properties.</rdfs:comment>
    <rdfs:comment xml:lang="sv">skos:prefLabel, skos:altLabel och skos:hiddenLabel är parvis åtskilda egenskaper.</rdfs:comment>
    <!-- For non-OWL aware applications -->
    <rdf:type rdf:resource="http://www.w3.org/1999/02/22-rdf-syntax-ns#Property"/>
  </rdf:Description>
  <rdf:Description rdf:about="#altLabel">
    <rdfs:label xml:lang="en">alternative label</rdfs:label>
    <rdfs:label xml:lang="sv">alternativ term</rdfs:label>
    <rdfs:isDefinedBy rdf:resource="http://www.w3.org/2004/02/skos/core"/>
    <skos:definition xml:lang="en">An alternative lexical label for a resource.</skos:definition>
    <skos:definition xml:lang="sv">En alternativ term för en resurs.</skos:definition>
    <skos:example xml:lang="en">Acronyms, abbreviations, spelling variants, and irregular plural/singular forms may be included among the alternative labels for a concept. Mis-spelled terms are normally included as hidden labels (see skos:hiddenLabel).</skos:example>
    <skos:example xml:lang="sv">Akronymer, förkortningar, alternativa stavningar och oregelbundna plural- och singularformer kan ingå bland alternativa termer för ett begrepp. Felstavningar anges vanligen som dolda termer (se skos:hiddenLabel).</skos:example>
    <!-- S10 -->
    <rdf:type rdf:resource="http://www.w3.org/2002/07/owl#AnnotationProperty"/>
    <!-- S11 -->
    <rdfs:subPropertyOf rdf:resource="http://www.w3.org/2000/01/rdf-schema#label"/>
    <!-- S12 (not formally stated) -->
    <rdfs:comment xml:lang="en">The range of skos:altLabel is the class of RDF plain literals.</rdfs:comment>
    <rdfs:comment xml:lang="sv">Omfattningen av skos:altLabel är klassen RDF plain literals.</rdfs:comment>
    <!-- S13 (not formally stated) -->
    <rdfs:comment xml:lang="en">skos:prefLabel, skos:altLabel and skos:hiddenLabel are pairwise disjoint properties.</rdfs:comment>
    <rdfs:comment xml:lang="sv">skos:prefLabel, skos:altLabel och skos:hiddenLabel är parvis åtskilda egenskaper.</rdfs:comment>
    <!-- For non-OWL aware applications -->
    <rdf:type rdf:resource="http://www.w3.org/1999/02/22-rdf-syntax-ns#Property"/>
  </rdf:Description>
  <rdf:Description rdf:about="#hiddenLabel">
    <rdfs:label xml:lang="en">hidden label</rdfs:label>
    <rdfs:label xml:lang="sv">dold term</rdfs:label>
    <rdfs:isDefinedBy rdf:resource="http://www.w3.org/2004/02/skos/core"/>
    <skos:definition xml:lang="en">A lexical label for a resource that should be hidden when generating visual displays of the resource, but should still be accessible to free text search operations.</skos:definition>
    <skos:definition xml:lang="sv">En term som bör döljas när man presenterar en resurs men som ska ingå som underlag för fritextsökningar.</skos:definition>
    <!-- S10 -->
    <rdf:type rdf:resource="http://www.w3.org/2002/07/owl#AnnotationProperty"/>
    <!-- S11 -->
    <rdfs:subPropertyOf rdf:resource="http://www.w3.org/2000/01/rdf-schema#label"/>
    <!-- S12 (not formally stated) -->
    <rdfs:comment xml:lang="en">The range of skos:hiddenLabel is the class of RDF plain literals.</rdfs:comment>
    <rdfs:comment xml:lang="sv">Omfattningen av skos:altLabel är klassen RDF plain literals.</rdfs:comment>
    <!-- S13 (not formally stated) -->
    <rdfs:comment xml:lang="en">skos:prefLabel, skos:altLabel and skos:hiddenLabel are pairwise disjoint properties.</rdfs:comment>
    <rdfs:comment xml:lang="sv">skos:prefLabel, skos:altLabel och skos:hiddenLabel är parvis åtskilda egenskaper.</rdfs:comment>
    <!-- For non-OWL aware applications -->
    <rdf:type rdf:resource="http://www.w3.org/1999/02/22-rdf-syntax-ns#Property"/>
  </rdf:Description>
  <rdf:Description rdf:about="#notation">
    <rdfs:label xml:lang="en">notation</rdfs:label>
    <rdfs:label xml:lang="sv">identifierare</rdfs:label>
    <rdfs:isDefinedBy rdf:resource="http://www.w3.org/2004/02/skos/core"/>
    <skos:definition xml:lang="en">A notation, also known as classification code, is a string of characters such as "T58.5" or "303.4833" used to uniquely identify a concept within the scope of a given concept scheme.</skos:definition>
    <skos:definition xml:lang="en">En identifierare eller kod är en uppsättning tecken som t.ex. "T58.5" eller "303.4833" och används för att unikt identifiera ett begrepp i en begreppsmodell.</skos:definition>
    <skos:scopeNote xml:lang="en">By convention, skos:notation is used with a typed literal in the object position of the triple.</skos:scopeNote>
    <skos:scopeNote xml:lang="sv">Vanligen används skos:notation i form av en typed literal som objekt i en trippel.</skos:scopeNote>
    <!-- S15 -->
    <rdf:type rdf:resource="http://www.w3.org/2002/07/owl#DatatypeProperty"/>
    <!-- For non-OWL aware applications -->
    <rdf:type rdf:resource="http://www.w3.org/1999/02/22-rdf-syntax-ns#Property"/>
  </rdf:Description>
  <rdf:Description rdf:about="#note">
    <rdfs:label xml:lang="en">note</rdfs:label>
    <rdfs:label xml:lang="sv">anmärkning</rdfs:label>
    <rdfs:isDefinedBy rdf:resource="http://www.w3.org/2004/02/skos/core"/>
    <skos:definition xml:lang="en">A general note, for any purpose.</skos:definition>
    <skos:definition xml:lang="sv">En allmän anmärkning i vilket syfte som helst.</skos:definition>
    <skos:scopeNote xml:lang="en">This property may be used directly, or as a super-property for more specific note types.</skos:scopeNote>
    <skos:scopeNote xml:lang="sv">Denna egenskap kan användas direkt eller som en överordnad egenskap för mer specifika anmärkningstyper.</skos:scopeNote>
    <!-- S16 -->
    <rdf:type rdf:resource="http://www.w3.org/2002/07/owl#AnnotationProperty"/>
    <!-- For non-OWL aware applications -->
    <rdf:type rdf:resource="http://www.w3.org/1999/02/22-rdf-syntax-ns#Property"/>
  </rdf:Description>
  <rdf:Description rdf:about="#changeNote">
    <rdfs:label xml:lang="en">change note</rdfs:label>
    <rdfs:label xml:lang="sv">förändringsanmärkning</rdfs:label>
    <rdfs:isDefinedBy rdf:resource="http://www.w3.org/2004/02/skos/core"/>
    <skos:definition xml:lang="en">A note about a modification to a concept.</skos:definition>
    <skos:definition xml:lang="sv">Anmärkning om förändringar av ett begrepp.</skos:definition>
    <!-- S16 -->
    <rdf:type rdf:resource="http://www.w3.org/2002/07/owl#AnnotationProperty"/>
    <!-- S17 -->
    <rdfs:subPropertyOf rdf:resource="#note"/>
    <!-- For non-OWL aware applications -->
    <rdf:type rdf:resource="http://www.w3.org/1999/02/22-rdf-syntax-ns#Property"/>
  </rdf:Description>
  <rdf:Description rdf:about="#definition">
    <rdfs:label xml:lang="en">definition</rdfs:label>
    <rdfs:label xml:lang="sv">definition</rdfs:label>
    <rdfs:isDefinedBy rdf:resource="http://www.w3.org/2004/02/skos/core"/>
    <skos:definition xml:lang="en">A statement or formal explanation of the meaning of a concept.</skos:definition>
    <skos:definition xml:lang="sv">En beskrivning eller förklaring av ett begrepps innebörd.</skos:definition>
    <!-- S16 -->
    <rdf:type rdf:resource="http://www.w3.org/2002/07/owl#AnnotationProperty"/>
    <!-- S17 -->
    <rdfs:subPropertyOf rdf:resource="#note"/>
    <!-- For non-OWL aware applications -->
    <rdf:type rdf:resource="http://www.w3.org/1999/02/22-rdf-syntax-ns#Property"/>
  </rdf:Description>
  <rdf:Description rdf:about="#editorialNote">
    <rdfs:label xml:lang="en">editorial note</rdfs:label>
    <rdfs:label xml:lang="sv">redaktionell anmärkning</rdfs:label>
    <rdfs:isDefinedBy rdf:resource="http://www.w3.org/2004/02/skos/core"/>
    <skos:definition xml:lang="en">A note for an editor, translator or maintainer of the vocabulary.</skos:definition>
    <skos:definition xml:lang="sv">Information avsedd för redaktör, översättare elleter förvaltare av begreppsmodellen.</skos:definition>
    <!-- S16 -->
    <rdf:type rdf:resource="http://www.w3.org/2002/07/owl#AnnotationProperty"/>
    <!-- S17 -->
    <rdfs:subPropertyOf rdf:resource="#note"/>
    <!-- For non-OWL aware applications -->
    <rdf:type rdf:resource="http://www.w3.org/1999/02/22-rdf-syntax-ns#Property"/>
  </rdf:Description>
  <rdf:Description rdf:about="#example">
    <rdfs:label xml:lang="en">example</rdfs:label>
    <rdfs:label xml:lang="sv">exempel</rdfs:label>
    <rdfs:isDefinedBy rdf:resource="http://www.w3.org/2004/02/skos/core"/>
    <skos:definition xml:lang="en">An example of the use of a concept.</skos:definition>
    <skos:definition xml:lang="sv">Exempel på hur ett begrepp kan användas.</skos:definition>
    <!-- S16 -->
    <rdf:type rdf:resource="http://www.w3.org/2002/07/owl#AnnotationProperty"/>
    <!-- S17 -->
    <rdfs:subPropertyOf rdf:resource="#note"/>
    <!-- For non-OWL aware applications -->
    <rdf:type rdf:resource="http://www.w3.org/1999/02/22-rdf-syntax-ns#Property"/>
  </rdf:Description>
  <rdf:Description rdf:about="#historyNote">
    <rdfs:label xml:lang="en">history note</rdfs:label>
    <rdfs:label xml:lang="sv">historisk anmärkning</rdfs:label>
    <rdfs:isDefinedBy rdf:resource="http://www.w3.org/2004/02/skos/core"/>
    <skos:definition xml:lang="en">A note about the past state/use/meaning of a concept.</skos:definition>
    <skos:definition xml:lang="sv">Information om tidigare status/användning/innebörd av ett begrepp.</skos:definition>
    <!-- S16 -->
    <rdf:type rdf:resource="http://www.w3.org/2002/07/owl#AnnotationProperty"/>
    <!-- S17 -->
    <rdfs:subPropertyOf rdf:resource="#note"/>
    <!-- For non-OWL aware applications -->
    <rdf:type rdf:resource="http://www.w3.org/1999/02/22-rdf-syntax-ns#Property"/>
  </rdf:Description>
  <rdf:Description rdf:about="#scopeNote">
    <rdfs:label xml:lang="en">scope note</rdfs:label>
    <rdfs:label xml:lang="sv">användningsanmärkning</rdfs:label>
    <rdfs:isDefinedBy rdf:resource="http://www.w3.org/2004/02/skos/core"/>
    <skos:definition xml:lang="en">A note that helps to clarify the meaning and/or the use of a concept.</skos:definition>
    <skos:definition xml:lang="sv">Information som förtydligar betyldelsen av och/eller användningen av ett begrepp.</skos:definition>
    <!-- S16 -->
    <rdf:type rdf:resource="http://www.w3.org/2002/07/owl#AnnotationProperty"/>
    <!-- S17 -->
    <rdfs:subPropertyOf rdf:resource="#note"/>
    <!-- For non-OWL aware applications -->
    <rdf:type rdf:resource="http://www.w3.org/1999/02/22-rdf-syntax-ns#Property"/>
  </rdf:Description>
  <rdf:Description rdf:about="#semanticRelation">
    <rdfs:label xml:lang="en">is in semantic relation with</rdfs:label>
    <rdfs:label xml:lang="sv">är semantiskt relaterat till</rdfs:label>
    <rdfs:isDefinedBy rdf:resource="http://www.w3.org/2004/02/skos/core"/>
    <skos:definition xml:lang="en">Links a concept to a concept related by meaning.</skos:definition>
    <skos:definition xml:lang="sv">Kopplar ihop två begrepp som har en meningsfull relation.</skos:definition>
    <skos:scopeNote xml:lang="en">This property should not be used directly, but as a super-property for all properties denoting a relationship of meaning between concepts.</skos:scopeNote>
    <skos:scopeNote xml:lang="sv">Denna egenskap ska inte användas direkt. Den är en abstrakt egenskap för de egenskaper som beskriver inbördes förhållanden mellan begrepp.</skos:scopeNote>
    <!-- S18 -->
    <rdf:type rdf:resource="http://www.w3.org/2002/07/owl#ObjectProperty"/>
    <!-- S19 -->
    <rdfs:domain rdf:resource="#Concept"/>
    <!-- S20 -->
    <rdfs:range rdf:resource="#Concept"/>
    <!-- For non-OWL aware applications -->
    <rdf:type rdf:resource="http://www.w3.org/1999/02/22-rdf-syntax-ns#Property"/>
  </rdf:Description>
  <rdf:Description rdf:about="#broader">
    <rdfs:label xml:lang="en">has broader</rdfs:label>
    <rdfs:label xml:lang="sv">har överordnat begrepp</rdfs:label>
    <rdfs:isDefinedBy rdf:resource="http://www.w3.org/2004/02/skos/core"/>
    <skos:definition xml:lang="en">Relates a concept to a concept that is more general in meaning.</skos:definition>
    <skos:definition xml:lang="sv">Kopplar samman ett begrepp med ett annat som är mer generellt definierat.</skos:definition>
    <rdfs:comment xml:lang="en">Broader concepts are typically rendered as parents in a concept hierarchy (tree).</rdfs:comment>
    <rdfs:comment xml:lang="sv">Överordnade begrepp visas vanligen som föräldrar i ett begreppsdiagram (träd).</rdfs:comment>
    <skos:scopeNote xml:lang="en">By convention, skos:broader is only used to assert an immediate (i.e. direct) hierarchical link between two conceptual resources.</skos:scopeNote>
    <skos:scopeNote xml:lang="sv">Vanligen används skos:broader enbart för direkta relationer mellan två begrepp.</skos:scopeNote>
    <!-- S18 -->
    <rdf:type rdf:resource="http://www.w3.org/2002/07/owl#ObjectProperty"/>
    <!-- S22 -->
    <rdfs:subPropertyOf rdf:resource="#broaderTransitive"/>
    <!-- S25 -->
    <owl:inverseOf rdf:resource="#narrower"/>
    <!-- For non-OWL aware applications -->
    <rdf:type rdf:resource="http://www.w3.org/1999/02/22-rdf-syntax-ns#Property"/>
  </rdf:Description>
  <rdf:Description rdf:about="#narrower">
    <rdfs:label xml:lang="en">has narrower</rdfs:label>
    <rdfs:label xml:lang="sv">har underordnat begrepp</rdfs:label>
    <rdfs:isDefinedBy rdf:resource="http://www.w3.org/2004/02/skos/core"/>
    <skos:definition xml:lang="en">Relates a concept to a concept that is more specific in meaning.</skos:definition>
    <skos:definition xml:lang="sv">Ett begrepp som har en mer specifik definition.</skos:definition>
    <skos:scopeNote xml:lang="en">By convention, skos:broader is only used to assert an immediate (i.e. direct) hierarchical link between two conceptual resources.</skos:scopeNote>
    <skos:scopeNote xml:lang="sv">Vanligtvis används skos:broader enbart för att uttrycka ett direkt hierarkiskt förhållande mellan två begrepp.</skos:scopeNote>
    <rdfs:comment xml:lang="en">Narrower concepts are typically rendered as children in a concept hierarchy (tree).</rdfs:comment>
    <rdfs:comment xml:lang="sv">Underordnade begrepp visas vanligen som barn i ett begreppsdiagram (träd).</rdfs:comment>
    <!-- S18 -->
    <rdf:type rdf:resource="http://www.w3.org/2002/07/owl#ObjectProperty"/>
    <!-- S22 -->
    <rdfs:subPropertyOf rdf:resource="#narrowerTransitive"/>
    <!-- S25 -->
    <owl:inverseOf rdf:resource="#broader"/>
    <!-- For non-OWL aware applications -->
    <rdf:type rdf:resource="http://www.w3.org/1999/02/22-rdf-syntax-ns#Property"/>
  </rdf:Description>
  <rdf:Description rdf:about="#related">
    <rdfs:label xml:lang="en">has related</rdfs:label>
    <rdfs:label xml:lang="sv">är relaterat med</rdfs:label>
    <rdfs:isDefinedBy rdf:resource="http://www.w3.org/2004/02/skos/core"/>
    <skos:definition xml:lang="en">Relates a concept to a concept with which there is an associative semantic relationship.</skos:definition>
    <skos:definition xml:lang="sv">Ett begrepp till vilket det finns en associativ begreppsrelation.</skos:definition>
    <!-- S18 -->
    <rdf:type rdf:resource="http://www.w3.org/2002/07/owl#ObjectProperty"/>
    <!-- S21 -->
    <rdfs:subPropertyOf rdf:resource="#semanticRelation"/>
    <!-- S23 -->
    <rdf:type rdf:resource="http://www.w3.org/2002/07/owl#SymmetricProperty"/>
    <!-- S27 (not formally stated) -->
    <rdfs:comment xml:lang="en">skos:related is disjoint with skos:broaderTransitive</rdfs:comment>
    <rdfs:comment xml:lang="sv">skos:related är åtskilt från skos:broaderTransitive</rdfs:comment>
    <!-- For non-OWL aware applications -->
    <rdf:type rdf:resource="http://www.w3.org/1999/02/22-rdf-syntax-ns#Property"/>
  </rdf:Description>
  <rdf:Description rdf:about="#broaderTransitive">
    <rdfs:label xml:lang="en">has broader transitive</rdfs:label>
    <rdfs:label xml:lang="sv">har transitivt överordnat begrepp</rdfs:label>
    <rdfs:isDefinedBy rdf:resource="http://www.w3.org/2004/02/skos/core"/>
    <skos:definition>skos:broaderTransitive is a transitive superproperty of skos:broader.</skos:definition>
    <skos:definition xml:lang="sv">skos:broaderTransitive är en transitiv överordnad egenskap för skos:broader.</skos:definition>
    <skos:scopeNote xml:lang="en">By convention, skos:broaderTransitive is not used to make assertions. Rather, the properties can be used to draw inferences about the transitive closure of the hierarchical relation, which is useful e.g. when implementing a simple query expansion algorithm in a search application.</skos:scopeNote>
    <skos:scopeNote xml:lang="sv">Vanligen används inte skos:broaderTransitive för påståenden. Istället kan dessa egenskaper användas för att härleda trasitiva egenskaper för en hierarkisk relation, t.ex. vid implementation av frågealgoritmer i sökapplikationer.</skos:scopeNote>
    <!-- S18 -->
    <rdf:type rdf:resource="http://www.w3.org/2002/07/owl#ObjectProperty"/>
    <!-- S21 -->
    <rdfs:subPropertyOf rdf:resource="#semanticRelation"/>
    <!-- S24 -->
    <rdf:type rdf:resource="http://www.w3.org/2002/07/owl#TransitiveProperty"/>
    <!-- S26 -->
    <owl:inverseOf rdf:resource="#narrowerTransitive"/>
    <!-- For non-OWL aware applications -->
    <rdf:type rdf:resource="http://www.w3.org/1999/02/22-rdf-syntax-ns#Property"/>
  </rdf:Description>
  <rdf:Description rdf:about="#narrowerTransitive">
    <rdfs:label xml:lang="en">has narrower transitive</rdfs:label>
    <rdfs:label xml:lang="sv">har transitivt underordnat begrepp</rdfs:label>
    <rdfs:isDefinedBy rdf:resource="http://www.w3.org/2004/02/skos/core"/>
    <skos:definition>skos:narrowerTransitive is a transitive superproperty of skos:narrower.</skos:definition>
    <skos:definition xml:lang="sv">skos:narrowerTransitive är en transitiv överordnad egenskap för skos:narrower.</skos:definition>
    <skos:scopeNote xml:lang="en">By convention, skos:narrowerTransitive is not used to make assertions. Rather, the properties can be used to draw inferences about the transitive closure of the hierarchical relation, which is useful e.g. when implementing a simple query expansion algorithm in a search application.</skos:scopeNote>
    <skos:scopeNote xml:lang="sv">Vanligen används inte skos:narrowerTransitive för påståenden. Istället kan dessa egenskaper användas för att härleda trasitiva egenskaper för en hierarkisk relation, t.ex. vid implementation av frågealgoritmer i sökapplikationer.</skos:scopeNote>
    <!-- S18 -->
    <rdf:type rdf:resource="http://www.w3.org/2002/07/owl#ObjectProperty"/>
    <!-- S21 -->
    <rdfs:subPropertyOf rdf:resource="#semanticRelation"/>
    <!-- S24 -->
    <rdf:type rdf:resource="http://www.w3.org/2002/07/owl#TransitiveProperty"/>
    <!-- S26 -->
    <owl:inverseOf rdf:resource="#broaderTransitive"/>
    <!-- For non-OWL aware applications -->
    <rdf:type rdf:resource="http://www.w3.org/1999/02/22-rdf-syntax-ns#Property"/>
  </rdf:Description>
  <rdf:Description rdf:about="#member">
    <rdfs:label xml:lang="en">has member</rdfs:label>
    <rdfs:label xml:lang="sv">har medlem</rdfs:label>
    <rdfs:isDefinedBy rdf:resource="http://www.w3.org/2004/02/skos/core"/>
    <skos:definition xml:lang="en">Relates a collection to one of its members.</skos:definition>
    <skos:definition xml:lang="sv">kopplar en samling till en medlem.</skos:definition>
    <!-- S30 -->
    <rdf:type rdf:resource="http://www.w3.org/2002/07/owl#ObjectProperty"/>
    <!-- S31 -->
    <rdfs:domain rdf:resource="#Collection"/>
    <!-- S32 -->
    <rdfs:range>
      <owl:Class>
	<owl:unionOf rdf:parseType="Collection">
	  <owl:Class rdf:about="#Concept"/>
	  <owl:Class rdf:about="#Collection"/>
	</owl:unionOf>
      </owl:Class>
    </rdfs:range>
    <!-- For non-OWL aware applications -->
    <rdf:type rdf:resource="http://www.w3.org/1999/02/22-rdf-syntax-ns#Property"/>
  </rdf:Description>
  <rdf:Description rdf:about="#memberList">
    <rdfs:label xml:lang="en">has member list</rdfs:label>
    <rdfs:label xml:lang="sv">har medlemsförteckning</rdfs:label>
    <rdfs:isDefinedBy rdf:resource="http://www.w3.org/2004/02/skos/core"/>
    <skos:definition xml:lang="en">Relates an ordered collection to the RDF list containing its members.</skos:definition>
    <skos:definition xml:lang="sv">Kopplar en ordnad samling begrepp till den RDF-lista som innehåller medlemmarna.</skos:definition>
    <!-- S30 -->
    <rdf:type rdf:resource="http://www.w3.org/2002/07/owl#ObjectProperty"/>
    <!-- S33 -->
    <rdfs:domain rdf:resource="#OrderedCollection"/>
    <!-- S35 -->
    <rdf:type rdf:resource="http://www.w3.org/2002/07/owl#FunctionalProperty"/>
    <!-- S34 -->
    <rdfs:range rdf:resource="http://www.w3.org/1999/02/22-rdf-syntax-ns#List"/>
    <!-- S36 (not formally stated) -->
    <rdfs:comment xml:lang="en">For any resource, every item in the list given as the value of the skos:memberList property is also a value of the skos:member property.</rdfs:comment>
    <rdfs:comment xml:lang="sv">För alla poster i listan som pekas ut i skos:memberList gäller att de även är värde för egenskapen skos:member.</rdfs:comment>
    <!-- For non-OWL aware applications -->
    <rdf:type rdf:resource="http://www.w3.org/1999/02/22-rdf-syntax-ns#Property"/>
  </rdf:Description>
  <rdf:Description rdf:about="#mappingRelation">
    <rdfs:label xml:lang="en">is in mapping relation with</rdfs:label>
    <rdfs:label xml:lang="sv">ingår i en jämförande relation till</rdfs:label>
    <rdfs:isDefinedBy rdf:resource="http://www.w3.org/2004/02/skos/core"/>
    <skos:definition xml:lang="en">Relates two concepts coming, by convention, from different schemes, and that have comparable meanings</skos:definition>
    <skos:definition xml:lang="sv">Kopplar samman två begrepp med likartad innebörd från olika begreppsmodeller.</skos:definition>
    <rdfs:comment xml:lang="en">These concept mapping relations mirror semantic relations, and the data model defined below is similar (with the exception of skos:exactMatch) to the data model defined for semantic relations. A distinct vocabulary is provided for concept mapping relations, to provide a convenient way to differentiate links within a concept scheme from links between concept schemes. However, this pattern of usage is not a formal requirement of the SKOS data model, and relies on informal definitions of best practice.</rdfs:comment>
    <rdfs:comment xml:lang="sv">Denna typ av relation speglar semantiska relationer och datamodellen nedan är liknar den för semantiska relationer (undantaget skos:exactMatch). En särskild vokabulär har skapats för att koppla samman begrepp vid jämförelser av deras innebörd med syfte att skilja på jämförelser inom en begreppsmodell och mellan begrepp i olika begreppsmodeller. Detta användningssätt krävs dock inte i SKOS datamodell utan bygger på praxis.</rdfs:comment>
    <!-- S38 -->
    <rdf:type rdf:resource="http://www.w3.org/2002/07/owl#ObjectProperty"/>
    <!-- S39 -->
    <rdfs:subPropertyOf rdf:resource="#semanticRelation"/>
    <!-- For non-OWL aware applications -->
    <rdf:type rdf:resource="http://www.w3.org/1999/02/22-rdf-syntax-ns#Property"/>
  </rdf:Description>
  <rdf:Description rdf:about="#broadMatch">
    <rdfs:label xml:lang="en">has broader match</rdfs:label>
    <rdfs:label xml:lang="sv">har överordnat motsvarande begrepp</rdfs:label>
    <rdfs:isDefinedBy rdf:resource="http://www.w3.org/2004/02/skos/core"/>
    <skos:definition xml:lang="en">skos:broadMatch is used to state a hierarchical mapping link between two conceptual resources in different concept schemes.</skos:definition>
    <skos:definition xml:lang="sv">skos:broadMatch används för att hierarkiskt relatera begrepp som ingår i olika begreppsmodeller.</skos:definition>
    <!-- S38 -->
    <rdf:type rdf:resource="http://www.w3.org/2002/07/owl#ObjectProperty"/>
    <!-- S40 -->
    <rdfs:subPropertyOf rdf:resource="#mappingRelation"/>
    <!-- S41 -->
    <rdfs:subPropertyOf rdf:resource="#broader"/>
    <!-- S43 -->
    <owl:inverseOf rdf:resource="#narrowMatch"/>
    <!-- For non-OWL aware applications -->
    <rdf:type rdf:resource="http://www.w3.org/1999/02/22-rdf-syntax-ns#Property"/>
  </rdf:Description>
  <rdf:Description rdf:about="#narrowMatch">
    <rdfs:label xml:lang="en">has narrower match</rdfs:label>
    <rdfs:label xml:lang="sv">har underordnat motsvarande begrepp</rdfs:label>
    <rdfs:isDefinedBy rdf:resource="http://www.w3.org/2004/02/skos/core"/>
    <skos:definition xml:lang="en">skos:narrowMatch is used to state a hierarchical mapping link between two conceptual resources in different concept schemes.</skos:definition>
    <skos:definition xml:lang="sv">skos:narrowMatch används för att hierarkiskt relatera begrepp som ingår i olika begreppsmodeller.</skos:definition>
    <!-- S38 -->
    <rdf:type rdf:resource="http://www.w3.org/2002/07/owl#ObjectProperty"/>
    <!-- S40 -->
    <rdfs:subPropertyOf rdf:resource="#mappingRelation"/>
    <!-- S41 -->
    <rdfs:subPropertyOf rdf:resource="#narrower"/>
    <!-- S43 -->
    <owl:inverseOf rdf:resource="#broadMatch"/>
    <!-- For non-OWL aware applications -->
    <rdf:type rdf:resource="http://www.w3.org/1999/02/22-rdf-syntax-ns#Property"/>
  </rdf:Description>
  <rdf:Description rdf:about="#relatedMatch">
    <rdfs:label xml:lang="en">has related match</rdfs:label>
    <rdfs:label xml:lang="sv">har relaterat motsvarande begrepp</rdfs:label>
    <rdfs:isDefinedBy rdf:resource="http://www.w3.org/2004/02/skos/core"/>
    <skos:definition xml:lang="en">skos:relatedMatch is used to state an associative mapping link between two conceptual resources in different concept schemes.</skos:definition>
    <skos:definition xml:lang="sv">skos:relatedMatch används för att uttrycka en associativ begreppsrelation mellan begrepp som ingår i olika begreppsmodeller.</skos:definition>
    <!-- S38 -->
    <rdf:type rdf:resource="http://www.w3.org/2002/07/owl#ObjectProperty"/>
    <!-- S40 -->
    <rdfs:subPropertyOf rdf:resource="#mappingRelation"/>
    <!-- S41 -->
    <rdfs:subPropertyOf rdf:resource="#related"/>
    <!-- S44 -->
    <rdf:type rdf:resource="http://www.w3.org/2002/07/owl#SymmetricProperty"/>
    <!-- For non-OWL aware applications -->
    <rdf:type rdf:resource="http://www.w3.org/1999/02/22-rdf-syntax-ns#Property"/>
  </rdf:Description>
  <rdf:Description rdf:about="#exactMatch">
    <rdfs:label xml:lang="en">has exact match</rdfs:label>
    <rdfs:label xml:lang="sv">har exakt motsvarande begrepp</rdfs:label>
    <rdfs:isDefinedBy rdf:resource="http://www.w3.org/2004/02/skos/core"/>
    <skos:definition xml:lang="en">skos:exactMatch is used to link two concepts, indicating a high degree of confidence that the concepts can be used interchangeably across a wide range of information retrieval applications. skos:exactMatch is a transitive property, and is a sub-property of skos:closeMatch.</skos:definition>
    <skos:definition xml:lang="sv">skos:exactMatch används för att koppla samman två begrepp där båda begreppen med största sannolikhet kan användas på samma sätt i informationsinsamlingssystem. skos:exactMatch är en transitiv egenskap och är en underliggande egenskap till skos:closeMatch.</skos:definition>
    <!-- S38 -->
    <rdf:type rdf:resource="http://www.w3.org/2002/07/owl#ObjectProperty"/>
    <!-- S42 -->
    <rdfs:subPropertyOf rdf:resource="#closeMatch"/>
    <!-- S44 -->
    <rdf:type rdf:resource="http://www.w3.org/2002/07/owl#SymmetricProperty"/>
    <!-- S45 -->
    <rdf:type rdf:resource="http://www.w3.org/2002/07/owl#TransitiveProperty"/>
    <!-- S46 (not formally stated) -->
    <rdfs:comment xml:lang="en">skos:exactMatch is disjoint with each of the properties skos:broadMatch and skos:relatedMatch.</rdfs:comment>
    <!-- For non-OWL aware applications -->
    <rdf:type rdf:resource="http://www.w3.org/1999/02/22-rdf-syntax-ns#Property"/>
  </rdf:Description>
  <rdf:Description rdf:about="#closeMatch">
    <rdfs:label xml:lang="en">has close match</rdfs:label>
    <rdfs:label xml:lang="sv">har snarlikt motsvarande begrepp</rdfs:label>
    <rdfs:isDefinedBy rdf:resource="http://www.w3.org/2004/02/skos/core"/>
    <skos:definition xml:lang="en">skos:closeMatch is used to link two concepts that are sufficiently similar that they can be used interchangeably in some information retrieval applications. In order to avoid the possibility of "compound errors" when combining mappings across more than two concept schemes, skos:closeMatch is not declared to be a transitive property.</skos:definition>
    <skos:definition xml:lang="sv">skos:closeMatch används för att koppla samman två begrepp som är tillräckligt lika för att kunna användas på liknande sätt i en del informationsinsamlingssystem. För att undvika risken med "aggregarade fel" i situationer där kopplingar skapats mellan begrepp i flera begreppsmodeller så är skos:closeMatch inte en transitiv egenskap.</skos:definition>
    <!-- S38 -->
    <rdf:type rdf:resource="http://www.w3.org/2002/07/owl#ObjectProperty"/>
    <!-- S40 -->
    <rdfs:subPropertyOf rdf:resource="#mappingRelation"/>
    <!-- S44 -->
    <rdf:type rdf:resource="http://www.w3.org/2002/07/owl#SymmetricProperty"/>
    <!-- For non-OWL aware applications -->
    <rdf:type rdf:resource="http://www.w3.org/1999/02/22-rdf-syntax-ns#Property"/>
  </rdf:Description>
</rdf:RDF>
